rupicola/io/ExamplesIO.fst
@@ -14,25 +14,33 @@ let apply_write_const : io unit = write true
 let apply_write : bool -> io unit = fun x -> write x
 
 let apply_io_bind_const : io bool =
-  io_bind (io_return true) (fun y -> io_return y)
+  let!@ x = return true in
+  return x
 
 let apply_io_bind_identity : bool -> io bool =
   fun x ->
-    io_bind (io_return x) (fun y -> io_return y)
+    let!@ y = return x in
+    return y
 
 let apply_io_bind_pure_if : bool -> io bool =
   fun x ->
-    io_bind (io_return x) (fun y -> if y then io_return false else io_return true)
+    if!@ (return x) then return false
+    else return true
 
 let apply_io_bind_write : bool -> io unit =
   fun x ->
-    io_bind (io_return x) (fun y -> write y)
+    let!@ y = return x in
+    write y
 
 let apply_io_bind_read_write : io unit =
-    io_bind (read ()) (fun y -> write y)
+  let!@ x = read () in
+  write x
 
 let apply_io_bind_read_write' : io unit =
-    io_bind (read ()) write
+  io_bind (read ()) write
 
 let apply_io_bind_read_if_write : io unit =
-    io_bind (read ()) (fun y -> if y then write false else write true)
+  let!@ x = read () in
+  if x
+  then write false
+  else write true
